src/Std/Data/Iterators/Producers/Slice.lean
@@ -23,5 +23,5 @@ Returns an iterator over the given slice. This iterator will emit the elements o
 in increasing order of the indices.
 -/
 @[always_inline, inline]
-def Std.Slice.iter [ToIterator (Slice γ) Id β] (s : Slice γ) :=
+def Std.Slice.iter [ToIterator (Slice γ) Id α β] (s : Slice γ) :=
   (Internal.iter s : Iter β)
