src/Std/Data/DTreeMap/Internal/Zipper.lean
@@ -368,9 +368,10 @@ public def Zipper.iter (t : Zipper α β) : Iter (α := Zipper α β) ((a : α) 
 public def Zipper.iterOfTree (t : Impl α β) : Iter (α := Zipper α β) ((a : α) × β a) :=
   Zipper.iter <| Zipper.done.prependMap t
 
-public instance : ToIterator (Zipper α β) Id ((a : α) × β a) where
-  State := Zipper α β
-  iterMInternal z := z.iter.toIterM
+@[inline, expose]
+public def Zipper.instToIterator :=
+  ToIterator.of (γ := Zipper α β) _ (fun z => z.iter)
+attribute [instance] Zipper.instToIterator
 
 @[simp]
 theorem Zipper.toList_done : (done : Zipper α β).toList = [] := rfl
@@ -684,9 +685,11 @@ public abbrev RicSlice α β [Ord α] := Slice (RicSliceData α β)
 public instance {α : Type u} {β : α → Type v} [Ord α] : Ric.Sliceable (Impl α β) α (RicSlice α β) where
   mkSlice carrier range := ⟨carrier, range⟩
 
-public instance [Ord α] : ToIterator (Slice (Internal.RicSliceData α β)) Id ((a : α) × β a) :=
-  ToIterator.of (RxcIterator α β)
+@[inline, expose]
+public def RicSlice.instToIterator {β : α → Type v} [Ord α] :=
+  ToIterator.of (γ := Slice (Internal.RicSliceData α β)) (β := ((a : α) × β a)) _
     (fun s => ⟨RxcIterator.mk (Zipper.prependMap s.1.treeMap Zipper.done) s.1.range.upper⟩)
+attribute [instance] RicSlice.instToIterator
 
 public theorem toList_ric {α : Type u} {β : α → Type v} [Ord α] [TransOrd α] (t : Impl α β)
     (ordered : t.Ordered) (bound : α) : t[*...=bound].toList = t.toList.filter (fun e => (compare e.fst bound).isLE) := by
@@ -712,9 +715,11 @@ public abbrev RicSlice α [Ord α] := Slice (RicSliceData α)
 public instance {α : Type u} [Ord α] : Ric.Sliceable (Impl α (fun _ => Unit)) α (Unit.RicSlice α) where
   mkSlice carrier range := ⟨carrier, range⟩
 
-public instance [Ord α] : ToIterator (Slice (RicSliceData α)) Id α :=
-  ToIterator.of _ fun s =>
+@[inline, expose]
+public def RicSlice.instToIterator [Ord α] :=
+  ToIterator.of (γ := Slice (RicSliceData α)) (β := α) _ fun s =>
     (⟨RxcIterator.mk (Zipper.prependMap s.1.treeMap Zipper.done) s.1.range.upper⟩ : Iter _ ).map fun e => (e.1)
+attribute [instance] RicSlice.instToIterator
 
 public theorem toList_ric {α : Type u} [Ord α] [TransOrd α] (t : Impl α (fun _ => Unit))
     (ordered : t.Ordered) (bound : α) : (t : Impl α (fun _ => Unit))[*...=bound].toList = (Internal.Impl.keys t).filter (fun e => (compare e bound).isLE) := by
@@ -744,9 +749,11 @@ public abbrev RicSlice α β [Ord α] := Slice (RicSliceData α β)
 public instance {α : Type u} {β : Type v} [Ord α] : Ric.Sliceable (Impl α (fun _ => β)) α (RicSlice α β) where
   mkSlice carrier range := ⟨carrier, range⟩
 
-public instance [Ord α] : ToIterator (Slice (RicSliceData α β)) Id (α × β) :=
-  ToIterator.of _ fun s =>
+@[inline, expose]
+public def RicSlice.instToIterator {β : Type v} [Ord α] :=
+  ToIterator.of (γ := Slice (RicSliceData α β)) _ fun s =>
     (⟨RxcIterator.mk (Zipper.prependMap s.1.treeMap Zipper.done) s.1.range.upper⟩ : Iter ((_ : α) × β)).map fun e => (e.1, e.2)
+attribute [instance] RicSlice.instToIterator
 
 public theorem toList_ric {α : Type u} {β : Type v} [Ord α] [TransOrd α] (t : Impl α (fun _ => β))
     (ordered : t.Ordered) (bound : α) : t[*...=bound].toList = (Internal.Impl.Const.toList t).filter (fun e => (compare e.fst bound).isLE) := by
@@ -776,9 +783,11 @@ public abbrev RioSlice α β [Ord α] := Slice (RioSliceData α β)
 public instance {α : Type u} {β : α → Type v} [Ord α] : Rio.Sliceable (Impl α β) α (RioSlice α β) where
   mkSlice carrier range := ⟨carrier, range⟩
 
-public instance [Ord α] : ToIterator (Slice (RioSliceData α β)) Id ((a : α) × β a) :=
-  ToIterator.of _ fun s =>
+@[inline, expose]
+public def RioSlice.instToIterator {β : α → Type v} [Ord α] :=
+  ToIterator.of (γ := Slice (RioSliceData α β)) (β := (a : α) × β a) _ fun s =>
     ⟨RxoIterator.mk (Zipper.prependMap s.1.treeMap Zipper.done) s.1.range.upper⟩
+attribute [instance] RioSlice.instToIterator
 
 public theorem toList_rio {α : Type u} {β : α → Type v} [Ord α] [TransOrd α] (t : Impl α β)
     (ordered : t.Ordered) (bound : α) : t[*...bound].toList = t.toList.filter (fun e => (compare e.fst bound).isLT) := by
@@ -804,9 +813,11 @@ public abbrev RioSlice α [Ord α] := Slice (RioSliceData α)
 public instance {α : Type u} [Ord α] : Rio.Sliceable (Impl α (fun _ => Unit)) α (Unit.RioSlice α) where
   mkSlice carrier range := ⟨carrier, range⟩
 
-public instance [Ord α] : ToIterator (Slice (RioSliceData α)) Id α :=
-  ToIterator.of _ fun s =>
+@[inline, expose]
+public def RioSlice.instToIterator [Ord α] :=
+  ToIterator.of (γ := Slice (RioSliceData α)) _ fun s =>
     (⟨RxoIterator.mk (Zipper.prependMap s.1.treeMap Zipper.done) s.1.range.upper⟩ : Iter _ ).map fun e => (e.1)
+attribute [instance] RioSlice.instToIterator
 
 public theorem toList_rio {α : Type u} [Ord α] [TransOrd α] (t : Impl α (fun _ => Unit))
     (ordered : t.Ordered) (bound : α) : (t : Impl α (fun _ => Unit))[*...<bound].toList = (Internal.Impl.keys t).filter (fun e => (compare e bound).isLT) := by
@@ -836,9 +847,11 @@ public abbrev RioSlice α β [Ord α] := Slice (RioSliceData α β)
 public instance {α : Type u} {β : Type v} [Ord α] : Rio.Sliceable (Impl α (fun _ => β)) α (RioSlice α β) where
   mkSlice carrier range := ⟨carrier, range⟩
 
-public instance [Ord α] : ToIterator (Slice (RioSliceData α β)) Id (α × β) :=
-  ToIterator.of _ fun s =>
+@[inline, expose]
+public def RioSlice.instToIterator {β : Type v} [Ord α] :=
+  ToIterator.of (γ := Slice (RioSliceData α β)) _ fun s =>
     (⟨RxoIterator.mk (Zipper.prependMap s.1.treeMap Zipper.done) s.1.range.upper⟩ : Iter ((_ : α) × β)).map fun e => (e.1, e.2)
+attribute [instance] RioSlice.instToIterator
 
 public theorem toList_rio {α : Type u} {β : Type v} [Ord α] [TransOrd α] (t : Impl α (fun _ => β))
     (ordered : t.Ordered) (bound : α) : t[*...<bound].toList = (Internal.Impl.Const.toList t).filter (fun e => (compare e.fst bound).isLT) := by
@@ -901,8 +914,11 @@ public abbrev RccSlice α β [Ord α] := Slice (RccSliceData α β)
 public instance {α : Type u} {β : α → Type v} [Ord α] : Rcc.Sliceable (Impl α β) α (RccSlice α β) where
   mkSlice carrier range := ⟨carrier, range⟩
 
-public instance [Ord α] : ToIterator (Slice (RccSliceData α β)) Id ((a : α) × β a) :=
-  ToIterator.of _ fun s => (rccIterator s.1.treeMap s.1.range.lower s.1.range.upper)
+@[inline, expose]
+public def RccSlice.instToIterator {β : α → Type v} [Ord α] :=
+  ToIterator.of (γ := Slice (RccSliceData α β)) (β := (a : α) × β a) _ fun s =>
+    (rccIterator s.1.treeMap s.1.range.lower s.1.range.upper)
+attribute [instance] RccSlice.instToIterator
 
 public theorem toList_rcc {α : Type u} {β : α → Type v} [Ord α] [TransOrd α] (t : Impl α β)
     (ordered : t.Ordered) (lowerBound upperBound : α) : t[lowerBound...=upperBound].toList = t.toList.filter (fun e => (compare e.fst lowerBound).isGE ∧ (compare e.fst upperBound).isLE) := by
@@ -925,9 +941,11 @@ public abbrev RccSlice α [Ord α] := Slice (RccSliceData α)
 public instance {α : Type u} [Ord α] : Rcc.Sliceable (Impl α (fun _ => Unit)) α (Unit.RccSlice α) where
   mkSlice carrier range := ⟨carrier, range⟩
 
-public instance [Ord α] : ToIterator (Slice (RccSliceData α)) Id α :=
-  ToIterator.of _ fun s =>
+@[inline, expose]
+public def RccSlice.instToIterator [Ord α] :=
+  ToIterator.of (γ := Slice (RccSliceData α)) _ fun s =>
     (⟨RxcIterator.mk (Zipper.prependMapGE s.1.treeMap s.1.range.lower .done) s.1.range.upper⟩ : Iter _ ).map fun e => (e.1)
+attribute [instance] RccSlice.instToIterator
 
 public theorem toList_rcc {α : Type u} [Ord α] [TransOrd α] (t : Impl α (fun _ => Unit))
     (ordered : t.Ordered) (lowerBound upperBound: α) : (t : Impl α (fun _ => Unit))[lowerBound...=upperBound].toList = (Internal.Impl.keys t).filter (fun e => (compare e lowerBound).isGE ∧ (compare e upperBound).isLE) := by
@@ -959,9 +977,11 @@ public abbrev RccSlice α β [Ord α] := Slice (RccSliceData α β)
 public instance {α : Type u} {β : Type v} [Ord α] : Rcc.Sliceable (Impl α (fun _ => β)) α (RccSlice α β) where
   mkSlice carrier range := ⟨carrier, range⟩
 
-public instance [Ord α] : ToIterator (Slice (RccSliceData α β)) Id (α × β) :=
-  ToIterator.of _ fun s =>
+@[inline, expose]
+public def RccSlice.instToIterator {β : Type v} [Ord α] :=
+  ToIterator.of (γ := Slice (RccSliceData α β)) _ fun s =>
     (⟨RxcIterator.mk (Zipper.prependMapGE s.1.treeMap s.1.range.lower .done) s.1.range.upper⟩ : Iter ((_ : α) × β)).map fun e => (e.1, e.2)
+attribute [instance] RccSlice.instToIterator
 
 public theorem toList_rcc {α : Type u} {β : Type v} [Ord α] [TransOrd α] (t : Impl α (fun _ => β))
     (ordered : t.Ordered) (lowerBound upperBound : α) : t[lowerBound...=upperBound].toList = (Internal.Impl.Const.toList t).filter (fun e => (compare e.fst lowerBound).isGE ∧ (compare e.fst upperBound).isLE) := by
@@ -1028,8 +1048,11 @@ public abbrev RcoSlice α β [Ord α] := Slice (RcoSliceData α β)
 public instance {α : Type u} {β : α → Type v} [Ord α] : Rco.Sliceable (Impl α β) α (RcoSlice α β) where
   mkSlice carrier range := ⟨carrier, range⟩
 
-public instance [Ord α] : ToIterator (Slice (RcoSliceData α β)) Id ((a : α) × β a) :=
-  ToIterator.of _ (fun s => rcoIterator s.1.treeMap s.1.range.lower s.1.range.upper)
+@[inline, expose]
+public def RcoSlice.instToIterator {β : α → Type v} [Ord α] :=
+  ToIterator.of (γ := Slice (RcoSliceData α β)) (β := (a : α) × β a) _ fun s =>
+    rcoIterator s.1.treeMap s.1.range.lower s.1.range.upper
+attribute [instance] RcoSlice.instToIterator
 
 public theorem toList_rco {α : Type u} {β : α → Type v} [Ord α] [TransOrd α] (t : Impl α β)
     (ordered : t.Ordered) (lowerBound upperBound : α) : t[lowerBound...<upperBound].toList = t.toList.filter (fun e => (compare e.fst lowerBound).isGE ∧ (compare e.fst upperBound).isLT) := by
@@ -1052,9 +1075,11 @@ public abbrev RcoSlice α [Ord α] := Slice (RcoSliceData α)
 public instance {α : Type u} [Ord α] : Rco.Sliceable (Impl α (fun _ => Unit)) α (Unit.RcoSlice α) where
   mkSlice carrier range := ⟨carrier, range⟩
 
-public instance [Ord α] : ToIterator (Slice (RcoSliceData α)) Id α :=
-  ToIterator.of _ fun s =>
+@[inline, expose]
+public def RcoSlice.instToIterator [Ord α] :=
+  ToIterator.of (γ := Slice (RcoSliceData α)) _ fun s =>
     (⟨RxoIterator.mk (Zipper.prependMapGE s.1.treeMap s.1.range.lower .done) s.1.range.upper⟩ : Iter _ ).map fun e => (e.1)
+attribute [instance] RcoSlice.instToIterator
 
 public theorem toList_rco {α : Type u} [Ord α] [TransOrd α] (t : Impl α (fun _ => Unit))
     (ordered : t.Ordered) (lowerBound upperBound: α) : (t : Impl α (fun _ => Unit))[lowerBound...<upperBound].toList = (Internal.Impl.keys t).filter (fun e => (compare e lowerBound).isGE ∧ (compare e upperBound).isLT) := by
@@ -1086,9 +1111,11 @@ public abbrev RcoSlice α β [Ord α] := Slice (RcoSliceData α β)
 public instance {α : Type u} {β : Type v} [Ord α] : Rco.Sliceable (Impl α (fun _ => β)) α (RcoSlice α β) where
   mkSlice carrier range := ⟨carrier, range⟩
 
-public instance [Ord α] : ToIterator (Slice (RcoSliceData α β)) Id (α × β) :=
-  ToIterator.of _ fun s =>
+@[inline, expose]
+public def RcoSlice.instToIterator {β : Type v} [Ord α] :=
+  ToIterator.of (γ := Slice (RcoSliceData α β)) _ fun s =>
     (⟨RxoIterator.mk (Zipper.prependMapGE s.1.treeMap s.1.range.lower .done) s.1.range.upper⟩ : Iter ((_ : α) × β)).map fun e => (e.1, e.2)
+attribute [instance] RcoSlice.instToIterator
 
 public theorem toList_rco {α : Type u} {β : Type v} [Ord α] [TransOrd α] (t : Impl α (fun _ => β))
     (ordered : t.Ordered) (lowerBound upperBound : α) : t[lowerBound...<upperBound].toList = (Internal.Impl.Const.toList t).filter (fun e => (compare e.fst lowerBound).isGE ∧ (compare e.fst upperBound).isLT) := by
@@ -1154,8 +1181,11 @@ public abbrev RooSlice α β [Ord α] := Slice (RooSliceData α β)
 public instance {α : Type u} {β : α → Type v} [Ord α] : Roo.Sliceable (Impl α β) α (RooSlice α β) where
   mkSlice carrier range := ⟨carrier, range⟩
 
-public instance [Ord α] : ToIterator (Slice (RooSliceData α β)) Id ((a : α) × β a) :=
-  ToIterator.of _ (fun s => rooIterator s.1.treeMap s.1.range.lower s.1.range.upper)
+@[inline, expose]
+public def RooSlice.instToIterator {β : α → Type v} [Ord α] :=
+  ToIterator.of (γ := Slice (RooSliceData α β)) (β := (a : α) × β a) _ fun s =>
+    rooIterator s.1.treeMap s.1.range.lower s.1.range.upper
+attribute [instance] RooSlice.instToIterator
 
 public theorem toList_roo {α : Type u} {β : α → Type v} [Ord α] [TransOrd α] (t : Impl α β)
     (ordered : t.Ordered) (lowerBound upperBound : α) : t[lowerBound<...<upperBound].toList = t.toList.filter (fun e => (compare e.fst lowerBound).isGT ∧ (compare e.fst upperBound).isLT) := by
@@ -1178,9 +1208,11 @@ public abbrev RooSlice α [Ord α] := Slice (RooSliceData α)
 public instance {α : Type u} [Ord α] : Roo.Sliceable (Impl α (fun _ => Unit)) α (Unit.RooSlice α) where
   mkSlice carrier range := ⟨carrier, range⟩
 
-public instance [Ord α] : ToIterator (Slice (RooSliceData α)) Id α :=
-  ToIterator.of _ fun s =>
+@[inline, expose]
+public def RooSlice.instToIterator [Ord α] :=
+  ToIterator.of (γ := Slice (RooSliceData α)) _ fun s =>
     (⟨RxoIterator.mk (Zipper.prependMapGT s.1.treeMap s.1.range.lower .done) s.1.range.upper⟩ : Iter _ ).map fun e => (e.1)
+attribute [instance] RooSlice.instToIterator
 
 public theorem toList_roo {α : Type u} [Ord α] [TransOrd α] (t : Impl α (fun _ => Unit))
     (ordered : t.Ordered) (lowerBound upperBound: α) : (t : Impl α (fun _ => Unit))[lowerBound<...<upperBound].toList = (Internal.Impl.keys t).filter (fun e => (compare e lowerBound).isGT ∧ (compare e upperBound).isLT) := by
@@ -1212,9 +1244,11 @@ public abbrev RooSlice α β [Ord α] := Slice (RooSliceData α β)
 public instance {α : Type u} {β : Type v} [Ord α] : Roo.Sliceable (Impl α (fun _ => β)) α (RooSlice α β) where
   mkSlice carrier range := ⟨carrier, range⟩
 
-public instance [Ord α] : ToIterator (Slice (RooSliceData α β)) Id (α × β) :=
-  ToIterator.of _ fun s =>
+@[inline, expose]
+public def RooSlice.instToIterator {β : Type v} [Ord α] :=
+  ToIterator.of (γ := Slice (RooSliceData α β)) _ fun s =>
     (⟨RxoIterator.mk (Zipper.prependMapGT s.1.treeMap s.1.range.lower .done) s.1.range.upper⟩ : Iter ((_ : α) × β)).map fun e => (e.1, e.2)
+attribute [instance] RooSlice.instToIterator
 
 public theorem toList_roo {α : Type u} {β : Type v} [Ord α] [TransOrd α] (t : Impl α (fun _ => β))
     (ordered : t.Ordered) (lowerBound upperBound : α) : t[lowerBound<...<upperBound].toList = (Internal.Impl.Const.toList t).filter (fun e => (compare e.fst lowerBound).isGT ∧ (compare e.fst upperBound).isLT) := by
@@ -1281,8 +1315,11 @@ public abbrev RocSlice α β [Ord α] := Slice (RocSliceData α β)
 public instance {α : Type u} {β : α → Type v} [Ord α] : Roc.Sliceable (Impl α β) α (RocSlice α β) where
   mkSlice carrier range := ⟨carrier, range⟩
 
-public instance [Ord α] : ToIterator (Slice (RocSliceData α β)) Id ((a : α) × β a) :=
-  ToIterator.of _ (fun s => rocIterator s.1.treeMap s.1.range.lower s.1.range.upper)
+@[inline, expose]
+public def RocSlice.instToIterator {β : α → Type v} [Ord α] :=
+  ToIterator.of (γ := Slice (RocSliceData α β)) (β := (a : α) × β a) _ fun s =>
+    rocIterator s.1.treeMap s.1.range.lower s.1.range.upper
+attribute [instance] RocSlice.instToIterator
 
 public theorem toList_roc {α : Type u} {β : α → Type v} [Ord α] [TransOrd α] (t : Impl α β)
     (ordered : t.Ordered) (lowerBound upperBound : α) : t[lowerBound<...=upperBound].toList = t.toList.filter (fun e => (compare e.fst lowerBound).isGT ∧ (compare e.fst upperBound).isLE) := by
@@ -1305,9 +1342,11 @@ public abbrev RocSlice α [Ord α] := Slice (RocSliceData α)
 public instance {α : Type u} [Ord α] : Roc.Sliceable (Impl α (fun _ => Unit)) α (Unit.RocSlice α) where
   mkSlice carrier range := ⟨carrier, range⟩
 
-public instance [Ord α] : ToIterator (Slice (RocSliceData α)) Id α :=
-  ToIterator.of _ fun s =>
+@[inline, expose]
+public def RocSlice.instToIterator [Ord α] :=
+  ToIterator.of (γ := Slice (RocSliceData α)) _ fun s =>
     (⟨RxcIterator.mk (Zipper.prependMapGT s.1.treeMap s.1.range.lower .done) s.1.range.upper⟩ : Iter _ ).map fun e => (e.1)
+attribute [instance] RocSlice.instToIterator
 
 public theorem toList_roc {α : Type u} [Ord α] [TransOrd α] (t : Impl α (fun _ => Unit))
     (ordered : t.Ordered) (lowerBound upperBound: α) : (t : Impl α (fun _ => Unit))[lowerBound<...=upperBound].toList = (Internal.Impl.keys t).filter (fun e => (compare e lowerBound).isGT ∧ (compare e upperBound).isLE) := by
@@ -1339,9 +1378,11 @@ public abbrev RocSlice α β [Ord α] := Slice (RocSliceData α β)
 public instance {α : Type u} {β : Type v} [Ord α] : Roc.Sliceable (Impl α (fun _ => β)) α (RocSlice α β) where
   mkSlice carrier range := ⟨carrier, range⟩
 
-public instance [Ord α] : ToIterator (Slice (RocSliceData α β)) Id (α × β) :=
-  ToIterator.of _ fun s =>
-  (⟨RxcIterator.mk (Zipper.prependMapGT s.1.treeMap s.1.range.lower .done) s.1.range.upper⟩ : Iter ((_ : α) × β)).map fun e => (e.1, e.2)
+@[inline, expose]
+public def RocSlice.instToIterator {β : Type v} [Ord α] :=
+  ToIterator.of (γ := Slice (RocSliceData α β)) _ fun s =>
+    (⟨RxcIterator.mk (Zipper.prependMapGT s.1.treeMap s.1.range.lower .done) s.1.range.upper⟩ : Iter ((_ : α) × β)).map fun e => (e.1, e.2)
+attribute [instance] RocSlice.instToIterator
 
 public theorem toList_roc {α : Type u} {β : Type v} [Ord α] [TransOrd α] (t : Impl α (fun _ => β))
     (ordered : t.Ordered) (lowerBound upperBound : α) : t[lowerBound<...=upperBound].toList = (Internal.Impl.Const.toList t).filter (fun e => (compare e.fst lowerBound).isGT ∧ (compare e.fst upperBound).isLE) := by
@@ -1393,8 +1434,11 @@ public abbrev RciSlice α β [Ord α] := Slice (RciSliceData α β)
 public instance {α : Type u} {β : α → Type v} [Ord α] : Rci.Sliceable (Impl α β) α (RciSlice α β) where
   mkSlice carrier range := ⟨carrier, range⟩
 
-public instance [Ord α] : ToIterator (Slice (RciSliceData α β)) Id ((a : α) × β a) :=
-  ToIterator.of _ (fun s => rciIterator s.1.treeMap s.1.range.lower)
+@[inline, expose]
+public def RciSlice.instToIterator {β : α → Type v} [Ord α] :=
+  ToIterator.of (γ := Slice (RciSliceData α β)) (β := (a : α) × β a) _ fun s =>
+    rciIterator s.1.treeMap s.1.range.lower
+attribute [instance] RciSlice.instToIterator
 
 public theorem toList_rci {α : Type u} {β : α → Type v} [Ord α] [TransOrd α] (t : Impl α β)
     (ordered : t.Ordered) (lowerBound : α) : t[lowerBound...*].toList = t.toList.filter (fun e => (compare e.fst lowerBound).isGE) := by
@@ -1417,9 +1461,11 @@ public abbrev RciSlice α [Ord α] := Slice (RciSliceData α)
 public instance {α : Type u} [Ord α] : Rci.Sliceable (Impl α (fun _ => Unit)) α (Unit.RciSlice α) where
   mkSlice carrier range := ⟨carrier, range⟩
 
-public instance [Ord α] : ToIterator (Slice (RciSliceData α)) Id α :=
-  ToIterator.of _ fun s =>
+@[inline, expose]
+public def RciSlice.instToIterator [Ord α] :=
+  ToIterator.of (γ := Slice (RciSliceData α)) _ fun s =>
     (⟨Zipper.prependMapGE s.1.treeMap s.1.range.lower Zipper.done⟩ : Iter _ ).map fun e => (e.1)
+attribute [instance] RciSlice.instToIterator
 
 public theorem toList_rci {α : Type u} [Ord α] [TransOrd α] (t : Impl α (fun _ => Unit))
     (ordered : t.Ordered) (lowerBound : α) : (t : Impl α (fun _ => Unit))[lowerBound...*].toList = (Internal.Impl.keys t).filter (fun e => (compare e lowerBound).isGE) := by
@@ -1454,9 +1500,11 @@ public abbrev RciSlice α β [Ord α] := Slice (RciSliceData α β)
 public instance {α : Type u} {β : Type v} [Ord α] : Rci.Sliceable (Impl α (fun _ => β)) α (RciSlice α β) where
   mkSlice carrier range := ⟨carrier, range⟩
 
-public instance [Ord α] : ToIterator (Slice (RciSliceData α β)) Id (α × β) :=
-  ToIterator.of _ fun s =>
+@[inline, expose]
+public def RciSlice.instToIterator {β : Type v} [Ord α] :=
+  ToIterator.of (γ := Slice (RciSliceData α β)) _ fun s =>
     (⟨(Zipper.prependMapGE s.1.treeMap s.1.range.lower Zipper.done)⟩ : Iter ((_ : α) × β)).map fun e => (e.1, e.2)
+attribute [instance] RciSlice.instToIterator
 
 public theorem toList_rci {α : Type u} {β : Type v} [Ord α] [TransOrd α] (t : Impl α (fun _ => β))
     (ordered : t.Ordered) (lowerBound : α) : t[lowerBound...*].toList = (Internal.Impl.Const.toList t).filter (fun e => (compare e.fst lowerBound).isGE) := by
@@ -1509,8 +1557,11 @@ public abbrev RoiSlice α β [Ord α] := Slice (RoiSliceData α β)
 public instance {α : Type u} {β : α → Type v} [Ord α] : Roi.Sliceable (Impl α β) α (RoiSlice α β) where
   mkSlice carrier range := ⟨carrier, range⟩
 
-public instance [Ord α] : ToIterator (Slice (RoiSliceData α β)) Id ((a : α) × β a) :=
-  ToIterator.of _ (fun s => roiIterator s.1.treeMap s.1.range.lower)
+@[inline, expose]
+public def RoiSlice.instToIterator {β : α → Type v} [Ord α] :=
+  ToIterator.of (γ := Slice (RoiSliceData α β)) (β := (a : α) × β a) _ fun s =>
+    roiIterator s.1.treeMap s.1.range.lower
+attribute [instance] RoiSlice.instToIterator
 
 public theorem toList_roi {α : Type u} {β : α → Type v} [Ord α] [TransOrd α] (t : Impl α β)
     (ordered : t.Ordered) (lowerBound : α) : t[lowerBound<...*].toList = t.toList.filter (fun e => (compare e.fst lowerBound).isGT) := by
@@ -1533,9 +1584,11 @@ public abbrev RoiSlice α [Ord α] := Slice (RoiSliceData α)
 public instance {α : Type u} [Ord α] : Roi.Sliceable (Impl α (fun _ => Unit)) α (Unit.RoiSlice α) where
   mkSlice carrier range := ⟨carrier, range⟩
 
-public instance [Ord α] : ToIterator (Slice (RoiSliceData α)) Id α :=
-  ToIterator.of _ fun s =>
+@[inline, expose]
+public def RoiSlice.instToIterator [Ord α] :=
+  ToIterator.of (γ := Slice (RoiSliceData α)) _ fun s =>
     (⟨Zipper.prependMapGT s.1.treeMap s.1.range.lower Zipper.done⟩ : Iter _ ).map fun e => (e.1)
+attribute [instance] RoiSlice.instToIterator
 
 public theorem toList_roi {α : Type u} [Ord α] [TransOrd α] (t : Impl α (fun _ => Unit))
     (ordered : t.Ordered) (lowerBound : α) : (t : Impl α (fun _ => Unit))[lowerBound<...*].toList = (Internal.Impl.keys t).filter (fun e => (compare e lowerBound).isGT) := by
@@ -1570,9 +1623,11 @@ public abbrev RoiSlice α β [Ord α] := Slice (RoiSliceData α β)
 public instance {α : Type u} {β : Type v} [Ord α] : Roi.Sliceable (Impl α (fun _ => β)) α (RoiSlice α β) where
   mkSlice carrier range := ⟨carrier, range⟩
 
-public instance [Ord α] : ToIterator (Slice (RoiSliceData α β)) Id (α × β) :=
-  ToIterator.of _ fun s =>
+@[inline, expose]
+public def RoiSlice.instToIterator {β : Type v} [Ord α] :=
+  ToIterator.of (γ := Slice (RoiSliceData α β)) _ fun s =>
     (⟨(Zipper.prependMapGT s.1.treeMap s.1.range.lower .done)⟩ : Iter ((_ : α) × β)).map fun e => (e.1, e.2)
+attribute [instance] RoiSlice.instToIterator
 
 public theorem toList_roi {α : Type u} {β : Type v} [Ord α] [TransOrd α] (t : Impl α (fun _ => β))
     (ordered : t.Ordered) (lowerBound : α) : t[lowerBound<...*].toList = (Internal.Impl.Const.toList t).filter (fun e => (compare e.fst lowerBound).isGT) := by
@@ -1619,8 +1674,11 @@ public abbrev RiiSlice α β := Slice (RiiSliceData α β)
 public instance {α : Type u} {β : α → Type v} : Rii.Sliceable (Impl α β) α (RiiSlice α β) where
   mkSlice carrier range := ⟨carrier, range⟩
 
-public instance : ToIterator (Slice (RiiSliceData α β)) Id ((a : α) × β a) :=
-  ToIterator.of _ (fun s => riiIterator s.1.treeMap)
+@[inline, expose]
+public def RiiSlice.instToIterator {β : α → Type v} :=
+  ToIterator.of (γ := Slice (RiiSliceData α β)) (β := (a : α) × β a) _ fun s =>
+    riiIterator s.1.treeMap
+attribute [instance] RiiSlice.instToIterator
 
 public theorem toList_rii {α : Type u} {β : α → Type v} (t : Impl α β) : t[*...*].toList = t.toList := by
   simp only [Rii.Sliceable.mkSlice, ← Slice.toList_iter, Slice.iter,
@@ -1641,9 +1699,11 @@ public abbrev RiiSlice α  := Slice (RiiSliceData α)
 public instance {α : Type u} : Rii.Sliceable (Impl α (fun _ => Unit)) α (Unit.RiiSlice α) where
   mkSlice carrier range := ⟨carrier, range⟩
 
-public instance : ToIterator (Slice (RiiSliceData α)) Id α :=
-  ToIterator.of _ fun s =>
+@[inline, expose]
+public def RiiSlice.instToIterator {α : Type u} :=
+  ToIterator.of (γ := Slice (RiiSliceData α)) _ fun s =>
     (⟨Zipper.prependMap s.internalRepresentation.treeMap .done⟩ : Iter _ ).map fun e => (e.1)
+attribute [instance] RiiSlice.instToIterator
 
 public theorem toList_rii {α : Type u} (t : Impl α (fun _ => Unit)) :
     (t : Impl α fun _ => Unit)[*...*].toList = Internal.Impl.keys t := by
@@ -1671,9 +1731,11 @@ public abbrev RiiSlice α β  := Slice (RiiSliceData α β)
 public instance {α : Type u} {β : Type v} : Rii.Sliceable (Impl α (fun _ => β)) α (Const.RiiSlice α β) where
   mkSlice carrier range := ⟨carrier, range⟩
 
-public instance : ToIterator (Slice (RiiSliceData α β)) Id (α × β) :=
-  ToIterator.of _ fun s =>
+@[inline, expose]
+public def RiiSlice.instToIterator {α : Type u} {β : Type v} :=
+  ToIterator.of (γ := Slice (RiiSliceData α β)) _ fun s =>
     (⟨Zipper.prependMap s.internalRepresentation.treeMap .done⟩ : Iter ((_ : α) × β)).map fun e => (e.1, e.2)
+attribute [instance] RiiSlice.instToIterator
 
 public theorem toList_rii {α : Type u} {β : Type v} (t : Impl α (fun _ => β)) :
     (t : Impl α fun _ => β)[*...*].toList = Internal.Impl.Const.toList t := by
